a bunch of work on actually proving the hoare rules for calc-mem-imp

Hoare/Hoare_Step.thy
@@ -19,30 +19,30 @@ begin
  * by playing the same parametricity trick as with the control languages?
  *)
 
-definition no_control_lifting :: "('a, 'b1, 'b2 :: {Bogus, Pord, Okay}) lifting \<Rightarrow>
-  ('a \<Rightarrow> 'b2 set) \<Rightarrow>
-  ('a, 'b1 , ('x, 'b2) control) lifting" where
-"no_control_lifting l S =
-  schem_lift NC (SP NX (SP NX (SINJ l S NC)))"
+definition no_control_lifting :: "('a, 'b1, 'b2 :: {Bogus, Pord}) lifting \<Rightarrow>
+  ('a, 'b1, ('x, 'b2) control) lifting" where
+"no_control_lifting l =
+  schem_lift NC (SP NX (SP NX (SINJ l NC)))"
 
-definition no_control_lifting_S ::"('a, 'b1, 'b2 :: {Bogus, Pord, Okay}) lifting \<Rightarrow>
+
+definition no_control_lifting_S ::"
+('a, 'b1, 'b2 :: {Bogus, Pord}) lifting \<Rightarrow>
   ('a \<Rightarrow> 'b2 set) \<Rightarrow>
   ('a \<Rightarrow> ('x, 'b2) control set)" where
 "no_control_lifting_S l S =
-  schem_lift_S NC (SP NX (SP NX (SINJ l S NC)))"
+  schem_lift_S NC (SP NX (SP NX (SINJS l S NC)))"
 
 (* something is weird with the pord constraint here. *)
 definition no_control_l :: "
 ('a, 'b1, 'b2 :: {Bogus, Pord, Okay}) lifting \<Rightarrow>
-  ('a \<Rightarrow> 'b2 set) \<Rightarrow>
 ('a \<Rightarrow> 'b1 \<Rightarrow> 'b1 :: {Bogus, Pord, Okay}) \<Rightarrow>
 ('a \<Rightarrow> ('x, 'b2 :: {Bogus, Pord, Okay}) control \<Rightarrow> ('x, 'b2 ) control)" where
-"no_control_l l S f =
-  lift_map_s id (no_control_lifting l S) f"
+"no_control_l l f =
+  lift_map_s id (no_control_lifting l) f"
 
 lemma no_control_l_valid :
   assumes H : "lifting_valid_ok l S"
-  shows "lifting_valid_ok (no_control_lifting l S) (no_control_lifting_S l S)"
+  shows "lifting_valid_ok (no_control_lifting l) (no_control_lifting_S l S)"
   using H
   unfolding no_control_lifting_def no_control_lifting_S_def schem_lift_defs schem_lift_S_defs
   by(fastforce intro: lifting_valid_fast lifting_ortho_fast
@@ -317,7 +317,7 @@ lemma HTS_imp_HT'' :
   assumes H: "f % {{P'}} (l' x) {{Q'}}"
   (* TODO: can we weaken this to lifting_valid_weak_ok *)
   assumes Valid : "lifting_valid_ok l S"
-  assumes Hf' : "f' = lift_map_t_s l' (no_control_lifting  l S) tg f"
+  assumes Hf' : "f' = lift_map_t_s l' (no_control_lifting  l) tg f"
   assumes H0 : "gs = pcomps fs"
   assumes Hpres : "sups_pres (set fs) (\<lambda> _ . ok_S)"
   assumes Hseq : "seq_sem_l_gen lfts \<in> set fs"
@@ -444,9 +444,9 @@ proof(rule HT'I)
 
         have Seq_pres : 
           "sups_pres {(seq_sem_l_gen lfts  ::('b \<Rightarrow> 'b gensyn list md_triv option md_prio \<times>
-            String.literal md_triv option md_prio \<times> 'c
+            String.literal option md_triv option md_prio \<times> 'c
             \<Rightarrow> 'b gensyn list md_triv option md_prio \<times>
-               String.literal md_triv option md_prio \<times>
+               String.literal option md_triv option md_prio \<times>
                'c))} (\<lambda> _ . ok_S)"
           using sups_pres_subset[OF Hpres, of "{(seq_sem_l_gen lfts )}"] Hseq
           by(auto)
@@ -478,7 +478,7 @@ proof(rule HT'I)
    but let's think about whether that will have unintended consequences.
  *)
         obtain pri1 pri2 rest where Msplit :
-          "m = (mdp pri1 (Some (mdt (G x z # c'))), mdp pri2 (Some (mdt (STR ''''))), rest)" and Rest : "rest \<in> ok_S"
+          "m = (mdp pri1 (Some (mdt (G x z # c'))), mdp pri2 (Some (mdt None)), rest)" and Rest : "rest \<in> ok_S"
           using Gs_alt' Dominate1 (*Dominate1_weak*) Skip Hpay Hcont Hf' Hpay_S
           by(auto simp add: seq_sem_l_gen_def seq_sem_lifting_gen_def 
             lift_pred_valid_ok_s_def lift_pred_noS_s_def lift_pred_s_def lift_map_s_def
@@ -595,5 +595,293 @@ proof(rule HT'I)
                   st = LUpd l (l' x) small_new old_big), npost-#}"
     by blast
 qed
+(*
+lemma HTS_imp_HT''' :
+  fixes fs :: "('b \<Rightarrow> ('b, 'c) control \<Rightarrow> ('b, 'c :: {Bogus, Mergeableb, Okay}) control) list"
+  assumes H: "f % {{P'}} (l' x) {{Q'}}"
+  (* TODO: can we weaken this to lifting_valid_weak_ok *)
+  assumes Valid : "lifting_valid_ok l S"
+  assumes Hf' : "f' = lift_map_t_s l' (no_control_lifting  l) tg f"
+  assumes H0 : "gs = pcomps fs"
+  assumes Hpres : "sups_pres (set fs) (\<lambda> _ . ok_S)"
+  assumes Hseq : "seq_sem_l_gen lfts \<in> set fs"
+  assumes Skip : "lfts x = Sskip"
+  assumes Active : "tg x = True"
+  assumes Xin : "x \<in> X"
+  assumes Hnemp : "g \<in> (set fs - {seq_sem_l_gen lfts})"
+  assumes Hdom : "(f' \<downharpoonleft> (set fs - {seq_sem_l_gen lfts}) X)"
+  assumes HP : "\<And> st . P st \<Longrightarrow> P' (LOut l (l' x) st)"
+
+  shows "|gs| {~ (\<lambda> st . P st) ~} [G x z] 
+    {~ (\<lambda> st . \<exists> old_big small_new . P old_big \<and> 
+        Q' small_new \<and> 
+        (\<exists> small_old . P' small_
+        st = LUpd l (l' x) small_new old_big) ~}"
+  (*shows "\<And> P1 . |gs| {~ P1 ~} [G c z] {~ (liftt_conc id l c P2 P1) ~}"*)
+proof(rule HT'I)
+  fix npost
+
+  interpret V : lifting_valid_ok l S
+    using Valid .
+
+  have "|#gs#| {#-(\<lambda>st. P st), (0 + npost)-#} [G x z] {#-(\<lambda>st. \<exists>old_big small_new.
+            P old_big \<and>
+            Q' small_new \<and>
+            st = LUpd l (l' x)  small_new old_big), npost-#}"
+    unfolding add_0
+  proof
+    fix c'
+
+    assume Guard : " |#gs#| {#(\<lambda>st. \<exists>old_big small_new.
+                            P old_big \<and>
+                            Q' small_new \<and>
+                            st =
+                            LUpd l (l' x) small_new
+                             old_big), npost#} c'"
+    show "|#gs#| {#P, npost#} ([G x z] @ c')"
+    proof
+      fix m :: "('b, 'c) control"
+      assume Ok : "m \<in> ok_S"
+      assume Hpay0 : "P (payload m)" and Hcont : "cont m = Inl ([G x z] @ c') "
+
+      show "safe_for gs m npost"
+      proof(cases "(sem_step gs m)")
+        case (Inr bad)
+  
+        then have False using Hcont H0
+          by(auto simp add: sem_step_def)
+  
+        then show ?thesis by auto
+      next
+        case (Inl m')
+
+        have Pres' : "sups_pres (set fs - {seq_sem_l_gen lfts}) (\<lambda> _ . ok_S)"
+          using sups_pres_subset[OF Hpres, of "set fs - {seq_sem_l_gen lfts}"] by auto
+
+        obtain fs_sub where Fs_sub : "set fs_sub = set fs - {seq_sem_l_gen lfts}"
+          using finite_list[of "set fs - {seq_sem_l_gen lfts}"]
+          by auto
+
+(* ok, so the idea now is:
+- we know full step (op + control flow) leads to m'
+- dominance over everything but the seq means we can treat it as
+  "op (dominant thing) then seq"
+- we can then unfold these things in order and everything should be ok.
+*)
+
+        have Assoc : 
+             "pcomps (fs_sub @ [seq_sem_l_gen lfts]) x m =
+              pcomps [pcomps fs_sub, pcomps [seq_sem_l_gen lfts]] x m"
+        proof(rule pcomps_assoc)
+
+          have "set fs - {seq_sem_l_gen lfts} \<union> set [seq_sem_l_gen lfts] = set fs"
+            using Hseq 
+            by(simp; blast)
+
+          then show "sups_pres (set fs_sub \<union> set [seq_sem_l_gen lfts]) (\<lambda> _ . ok_S)"
+            unfolding Fs_sub
+            using Hpres
+            by auto
+        next
+
+          have "set fs_sub \<noteq> {}" using Hnemp unfolding Fs_sub by auto
+
+          then show "fs_sub \<noteq> []" by auto
+        next
+
+          show "[seq_sem_l_gen lfts] \<noteq> []" by simp
+        next
+          show "m \<in> ok_S"
+            using Ok .
+        qed
+
+        have Set_alt : "set (fs_sub @ [seq_sem_l_gen lfts]) = set fs"
+          unfolding set_append Fs_sub
+          using Un_Diff_cancel2 Hseq
+          by auto
+
+        have Gs_alt : "gs x m = pcomps (fs_sub @ [seq_sem_l_gen lfts]) x m"
+          using pcomps_set_eq[OF Hpres Hseq _ Set_alt Ok, of fs] H0
+          by auto
+
+        have Hpay : "P (payload m)"
+          using Hpay0
+          by auto
+
+        then have Hpay_S : "payload m \<in> ok_S"
+          using Ok by(cases m; auto simp add: prod_ok_S)
+
+        have Hpay1' : "LOut l (l' x) (payload m) = LOut l (l' x) (payload m) \<and> P (payload m)"
+          using Hpay
+          by simp
+
+      have Hpay' : "Q' (f (l' x) (LOut l (l' x) (payload m)))"
+        using HTSE[OF H ] HP[OF Hpay]
+        by auto
+
+  (*
+        then have Hpay1 : "\<exists>full. LOut l (id c) full = LOut l c (payload m) \<and> P1 full" using Hpay_S
+          by auto
+
+        have Hpay' : " P2 (\<lambda>st. \<exists>full. LOut l (id c) full = st \<and> P1 full) (f c (LOut l c (payload m)))"
+          using HTSE[OF H ] Hpay1
+          by auto
+*)
+(* TODO: find a better solution than this awful type annotation hack *)
+
+        have Seq_pres : 
+          "sups_pres {(seq_sem_l_gen lfts  ::('b \<Rightarrow> 'b gensyn list md_triv option md_prio \<times>
+            String.literal option md_triv option md_prio \<times> 'c
+            \<Rightarrow> 'b gensyn list md_triv option md_prio \<times>
+               String.literal option md_triv option md_prio \<times>
+               'c))} (\<lambda> _ . ok_S)"
+          using sups_pres_subset[OF Hpres, of "{(seq_sem_l_gen lfts )}"] Hseq
+          by(auto)
+
+        have Gs_alt' : "gs x m = pcomps [pcomps fs_sub, seq_sem_l_gen lfts] x m"
+          using Gs_alt pcomps_singleton[OF Seq_pres _ Ok, of "[seq_sem_l_gen lfts]"]
+          unfolding Assoc
+          unfolding append.simps H0
+          by auto
+
+        have Hdom' :  "f' \<downharpoonleft> (set fs_sub) X"
+          using Fs_sub Hdom by auto
+
+        have Dominate1 : "pcomps fs_sub x m = f' x m"
+          using dominant_pcomps[OF Pres'[unfolded sym[OF Fs_sub]] Hnemp[unfolded sym[OF Fs_sub]] Hdom' Xin Ok]
+          by auto
+(*
+        (* Can we weaken our definition of dominant? *)
+        have Dominate1_weak :
+          "LOut (no_control_lifting l) (l' x) (pcomps fs_sub x m) =
+           LOut (no_control_lifting l) (l' x) (f' x m)"
+          sorry
+*)
+
+(* YOU ARE HERE. *)
+(* problem: seems like we still need to know something about the validity of the initial state.
+   maybe this is OK, but i worry that it will create problems.
+   the obvious solution is just to throw the validity condition into the pre and post conditions.
+   but let's think about whether that will have unintended consequences.
+ *)
+        obtain pri1 pri2 rest where Msplit :
+          "m = (mdp pri1 (Some (mdt (G x z # c'))), mdp pri2 (Some (mdt None)), rest)" and Rest : "rest \<in> ok_S"
+          using Gs_alt' Dominate1 (*Dominate1_weak*) Skip Hpay Hcont Hf' Hpay_S
+          by(auto simp add: seq_sem_l_gen_def seq_sem_lifting_gen_def 
+            lift_pred_valid_ok_s_def lift_pred_noS_s_def lift_pred_s_def lift_map_s_def
+            no_control_lifting_def cont_def
+            schem_lift_defs fst_l_def snd_l_def prio_l_def triv_l_def option_l_def seq_sem_def
+            prod_bsup no_control_l_def
+            split: md_prio.splits prod.splits md_triv.splits option.splits list.split_asm if_splits)
+
+        have Rest' : "rest \<in> S (l' x)"
+          using V.ok_S_valid Rest by auto
+
+        have LUpd_rest1 :
+          "rest <[ LUpd l (l' x) (f (l' x) (LOut l (l' x) rest)) rest"
+          using 
+            V.get_put
+          by auto
+
+        have LUpd_rest2 : "[^ LUpd l (l' x) (f (l' x) (LOut l (l' x) rest)) rest, rest ^] = LUpd l (l' x) (f (l' x) (LOut l (l' x) rest)) rest"
+          using bsup_base_leq2[OF LUpd_rest1]
+          by simp
+
+(*
+        then have LOut_m : 
+          "LOut (l_synt l' (no_control_lifting l)) x (gs x m) = LOut (l_synt l' (no_control_lifting l)) x (f' x m)"
+          using Gs_alt' Dominate1 Skip Hpay Hcont Hf' Msplit
+          unfolding l_synt_def
+          by(auto simp add: seq_sem_l_gen_def seq_sem_lifting_gen_def 
+            lift_pred_valid_s_def lift_pred_s_def
+            no_control_lifting_def cont_def
+            schem_lift_defs fst_l_def snd_l_def prio_l_def triv_l_def option_l_def seq_sem_def
+            prod_bsup no_control_l_def
+            split: md_prio.splits prod.splits md_triv.splits option.splits list.split_asm)
+*)
+
+(* key sub-result. *)
+
+(* key sub-result. idea here is that no_control_l means we won't overwrite. *)
+        have Cont_final : "cont m' = cont (seq_sem_l_gen lfts x m)"
+          using Hcont Msplit Skip Inl Gs_alt' Dominate1 Hf' Msplit
+          by(auto simp add: seq_sem_l_gen_def seq_sem_lifting_gen_def sem_step_def
+            lift_pred_s_def lift_map_s_def lift_map_t_s_def
+            no_control_lifting_def cont_def
+            schem_lift_defs fst_l_def snd_l_def prio_l_def triv_l_def option_l_def seq_sem_def
+            prod_bsup no_control_l_def prio_bsup option_bsup leq_refl triv_bsup split: md_prio.splits if_splits md_triv.splits option.splits)
+(*
+            split: md_prio.splits prod.splits md_triv.splits option.splits list.split_asm)         
+*)
+        hence Cont_final' : "cont m' = Inl c'"
+          using Hcont Msplit Skip
+          by(auto simp add: seq_sem_l_gen_def seq_sem_lifting_gen_def sem_step_def
+            lift_map_s_def lift_pred_s_def
+            no_control_lifting_def cont_def
+            schem_lift_defs fst_l_def snd_l_def prio_l_def triv_l_def option_l_def seq_sem_def
+            prod_bsup no_control_l_def
+            split: md_prio.splits prod.splits md_triv.splits option.splits list.split_asm)
+
+        have Pay_final : "payload m' = LUpd l (l' x) (f (l' x) (LOut l (l' x) (payload m))) (payload m)"
+          using Gs_alt' Dominate1 Skip Hpay Hcont Hf' Msplit Inl LUpd_rest2 Active
+          by(auto simp add: seq_sem_l_gen_def seq_sem_lifting_gen_def sem_step_def
+            lift_map_s_def lift_map_t_s_def lift_pred_s_def
+            no_control_lifting_def cont_def
+            schem_lift_defs fst_l_def snd_l_def prio_l_def triv_l_def option_l_def seq_sem_def
+            prod_bsup no_control_l_def
+            split: md_prio.splits prod.splits md_triv.splits option.splits list.split_asm)
+
+
+        have "(P (payload m)) \<and> Q' ((f (l' x) (LOut l (l' x) (payload m)))) \<and>
+              payload m' = LUpd l (l' x) (f (l' x) (LOut l (l' x) (payload m)))(payload m)"
+          using Hpay' Pay_final Hpay_S Hpay
+          by(auto)
+
+        then have Guard_Hyp : "\<exists>old_big small_new.
+             P old_big \<and>
+             Q' small_new \<and>
+             payload m' = LUpd l (l' x) small_new old_big"
+          by auto
+
+        have M'_ok : "m' \<in> ok_S"
+          using Hcont Msplit Skip Inl Gs_alt' Dominate1 Hf' Msplit Cont_final' Pay_final
+            V.ok_S_put[OF Rest]
+          by(auto simp add: seq_sem_l_gen_def seq_sem_lifting_gen_def sem_step_def
+            lift_pred_s_def lift_map_s_def lift_map_t_s_def
+            no_control_lifting_def cont_def
+            schem_lift_defs fst_l_def snd_l_def prio_l_def triv_l_def option_l_def seq_sem_def
+            prod_bsup no_control_l_def prio_bsup option_bsup leq_refl triv_bsup
+            prod_ok_S triv_ok_S prio_ok_S option_ok_S
+            split: md_prio.splits if_splits md_triv.splits option.splits)
+
+        have Conc' : "safe_for gs m' npost"
+          using guardediD[OF Guard, of "m'"]  Cont_final' Guard_Hyp
+          using M'_ok
+          unfolding Pay_final Cont_final' lift_pred_s_def lift_pred_s_def lift_pred_valid_ok_s_def
+            liftt_conc_def
+          
+          (*using lifting_validDO[OF Valid'] lifting_validDP[OF Valid'] lifting_validxDP'[OF Valid ]*)
+          by(cases m; auto)
+
+        have Inl_alt : "sem_step_p gs m m'"
+          using Inl unfolding sem_step_p_eq by simp
+
+        show  "safe_for gs m npost"
+          using safe_for_weaken[OF safe_for_extend[OF Conc' Excp_1[OF Inl_alt]], of npost]
+          by simp
+      qed
+    qed
+  qed
+
+  thus "\<exists>npre.
+          |#gs#| {#-P, (npre +
+                        npost)-#} [G x
+  z] {#-(\<lambda>st. \<exists>old_big small_new.
+                  P old_big \<and>
+                  Q' small_new \<and>
+                  st = LUpd l (l' x) small_new old_big), npost-#}"
+    by blast
+qed
+*)
 
 end
